Add in the RefChange dilemma

RefChange.fst
@@ -15,3 +15,28 @@ let whut (a:ref int) =
   assert (h0 =!= h1)
 
 // Turns out, this happens due to not annotating the top level terms. Seems like lots of weird top-level specific behaviour goes on...
+
+
+// Anyways, for what I really wanted to test:
+
+let foo (a:ref (ref int)) : St unit =
+  let b = !a in
+  !a := 5;
+  let c = !a in
+  assert (b == c \/ b =!= c); // this passes
+  // assert (b == c); // this fails; shouldn't this be true?
+  // assert (b =!= c); // this fails
+  ()
+
+// Looking at https://github.com/FStarLang/FStar/wiki/F*-Heap-Model
+// it seems like comparing addr_of would be more useful
+
+let bar (a:ref (ref int)) : St unit =
+  let a0 = a in
+  let a_deref_0 = !a in
+  !a := 5;
+  let a1 = a in
+  let a_deref_1 = !a in
+  assert (addr_of a0 == addr_of a1); // passes as expected
+  // assert (addr_of a_deref_0 == addr_of a_deref_1); // fails; shouldn't this be true?
+  ()
